Updated many proofs, added assignment equivalences

src/cnf/clause.lean
@@ -7,11 +7,16 @@ Carnegie Mellon Univeristy
 -/
 
 import cnf.literal
+import cnf.assignment
 import basic
 import data.nat.basic
+import init.data.nat.lemmas
 import data.list.basic
 import data.list.nodup
 import data.list.perm
+
+import data.finset.basic
+import init.logic
 
 /- (Disjunctive) clauses are lists of literals, joined by logical ORs. -/
 def clause := list literal
@@ -20,6 +25,8 @@ namespace clause
 
 open literal
 open list
+
+/-! # Properties, borrowed from lists -/
 
 instance : inhabited clause := ⟨[default literal]⟩
 
@@ -38,7 +45,7 @@ instance has_decidable_eq [s : decidable_eq literal] : decidable_eq clause
   end
 
 instance : has_mem literal clause := ⟨list.mem⟩
-instance : has_emptyc clause := ⟨list.nil⟩
+instance : has_emptyc clause := ⟨list.nil⟩ -- Refactor empty into [] below?
 instance : has_union clause := ⟨list.union⟩
 instance : has_inter clause := ⟨list.inter⟩
 instance : has_singleton literal clause := ⟨λ l, [l]⟩ 
@@ -46,75 +53,134 @@ instance : has_insert literal clause := ⟨list.insert⟩
 instance : has_append clause := ⟨list.append⟩
 instance : has_subset clause := ⟨list.subset⟩
 
+/-! # Evaluation under assignment -/
+
 /- The clause represents a disjunction, so we evaluate literals until tt is found -/
-def eval (α : assignment) (c : clause) : bool :=
+protected def eval (α : assignment) (c : clause) : bool :=
   c.foldr (λ l b, b || (l.eval α)) ff
 
-@[simp] theorem eval_nil (α : assignment) : eval α [] = ff := rfl
+-- Proving properties of the fold operation
+lemma eval_op_left_comm (α : assignment) : 
+  left_commutative (λ (l : literal) (b : bool), b || (literal.eval α l)) :=
+assume l₁ l₂ b, by simp [bool.bor_comm, bool.bor_assoc]
 
-@[simp] theorem eval_singleton (α : assignment) (l : literal) : eval α [l] = literal.eval α l :=
-by simp [eval]
+@[simp] theorem eval_nil (α : assignment) : clause.eval α [] = ff := rfl
 
-theorem eval_cons (α : assignment) (l : literal) (c : clause) : eval α (l :: c) = (literal.eval α l) || (eval α c) :=
-by simp [eval, bool.bor_comm]
+@[simp] theorem eval_singleton (α : assignment) (l : literal) : clause.eval α [l] = literal.eval α l :=
+by simp [clause.eval]
 
--- Can be cleaned up
-theorem eval_tt_iff_exists_literal_tt {α : assignment} {c : clause} : eval α c = tt ↔ ∃ l ∈ c, literal.eval α l = tt :=
+theorem eval_cons (α : assignment) (l : literal) (c : clause) : 
+  clause.eval α (l :: c) = (literal.eval α l) || (clause.eval α c) :=
+by simp [clause.eval, bool.bor_comm]
+
+theorem ne_nil_of_eval_tt {α : assignment} {c : clause} : clause.eval α c = tt → c ≠ [] :=
+by { contrapose, simp, intro h, simp [h] }
+
+lemma exists_literal_eval_tt_of_eval_tt {α : assignment} {c : clause} :
+  clause.eval α c = tt → ∃ l ∈ c, literal.eval α l = tt :=
 begin
   induction c with l ls ih,
-  { simp }, split,
-  { simp [eval_cons],
-    rintros (hl | hls),
-    { use l, simp [hl] },
-    { rcases ih.mp hls with ⟨l, hl, hlt⟩,
-      use l,
-      simp [hl, hlt] } },
-  { rintros ⟨l2, hl2, hlt⟩,
-    rcases eq_or_ne_mem_of_mem hl2 with rfl | ⟨hne, hls⟩,
-    { simp [eval_cons, hlt] },
-    { simp [eval_cons], 
-      have : ∃ (l3 : literal) (H : l3 ∈ ls), literal.eval α l3 = tt,  -- Shorten this?
-        { use l2, simp [hls, hlt] },
-      simp [ih.mpr this] } }
+  { contradiction },
+  { intro h,
+    simp [eval_cons] at h,
+    cases h,
+    { use [l, h] },
+    { rcases ih h with ⟨l₂, hl, he⟩,
+      use [l₂, mem_cons_of_mem l hl, he] } }
 end
 
--- Can be cleaned up
-theorem eval_ff_iff_literals_ff {α : assignment} {c : clause} : eval α c = ff ↔ ∀ l ∈ c, literal.eval α l = ff :=
+lemma eval_tt_of_exists_literal_eval_tt {α : assignment} {c : clause} :
+  (∃ l ∈ c, literal.eval α l = tt) → clause.eval α c = tt :=
 begin
-  induction c with l ls ih,
-  { simp }, split,
-  { simp [eval_cons],
-    intros hl hls,
-    exact and.intro hl (ih.mp hls) },
-  { intro hl,
-    simp [eval_cons],
-    simp [hl l (mem_cons_self l ls)],
-    have : ∀ (l2 : literal), l2 ∈ ls → literal.eval α l2 = ff,
-      { intros l2 hl2,
-        have : l2 ∈ l :: ls, from mem_cons_of_mem l hl2,
-        exact hl l2 this },
-    exact ih.mpr this }
+  rintros ⟨l, hl, he⟩,
+  induction c with d ds ih,
+  { exact absurd hl (not_mem_nil _) },
+  { rcases eq_or_ne_mem_of_mem hl with rfl | ⟨hne, hds⟩,
+    { simp [eval_cons, he] },
+    { simp [eval_cons, ih hds] } }
 end
 
--- TODO can be shortened, instead of four casework (I think)
-theorem eval_tautology (α : assignment) {c : clause} {l : literal} : l ∈ c → l.flip ∈ c → eval α c = tt :=
+theorem eval_tt_iff_exists_literal_eval_tt {α : assignment} {c : clause} : 
+  clause.eval α c = tt ↔ ∃ l ∈ c, literal.eval α l = tt :=
+⟨exists_literal_eval_tt_of_eval_tt, eval_tt_of_exists_literal_eval_tt⟩
+
+lemma forall_literal_eval_ff_of_mem_of_eval_ff {α : assignment} {c : clause} :
+  clause.eval α c = ff → ∀ l ∈ c, literal.eval α l = ff :=
 begin
-  rcases list_by_cases c with rfl | ⟨d, ds, rfl⟩,
+  induction c with d ds ih,
   { simp },
-  { intros hl hlf,
-    rcases bool_by_cases (α l.var) with h | h;
-    rcases exists_nat_of_lit l with ⟨n, (rfl | rfl)⟩;
-    simp [var, literal.flip] at h hl hlf;
-    apply eval_tt_iff_exists_literal_tt.mpr,
-    { use (Pos n),
-      simp [hl, hlf, h, literal.eval] },
-    { use (Pos n),
-      simp [hl, hlf, h, literal.eval] },
-    { use (Neg n),
-      simp [hl, hlf, h, literal.eval] },
-    { use (Neg n),
-      simp [hl, hlf, h, literal.eval] } }
+  { simp [eval_cons],
+    intros hl hds,
+    exact and.intro hl (ih hds) }
 end
+
+lemma eval_ff_of_forall_literal_eval_ff {α : assignment} {c : clause} :
+  (∀ l ∈ c, literal.eval α l = ff) → clause.eval α c = ff :=
+begin
+  induction c with l ls ih,
+  { simp },
+  { intro h,
+    simp [eval_cons, h l (mem_cons_self l ls)],
+    have : ∀ (m : literal), m ∈ ls → literal.eval α m = ff,
+    { intros m hm, exact h m (mem_cons_of_mem l hm) },
+    exact ih this }
+end
+
+theorem eval_ff_iff_forall_literal_eval_ff {α : assignment} {c : clause} : 
+  clause.eval α c = ff ↔ ∀ l ∈ c, literal.eval α l = ff :=
+⟨forall_literal_eval_ff_of_mem_of_eval_ff, eval_ff_of_forall_literal_eval_ff⟩
+
+theorem eval_tautology {c : clause} {l : literal} : 
+  l ∈ c → l.flip ∈ c → ∀ (α : assignment), clause.eval α c = tt :=
+begin
+  intros hl hlf α,
+  apply eval_tt_iff_exists_literal_eval_tt.mpr,
+  cases h : (literal.eval α l),
+  { use [l.flip, hlf, eval_flip_of_eval h] },
+  { use [l, hl, h] }
+end
+
+-- From a set POV, similarity becomes moot
+theorem eval_sim (α : assignment) {c₁ c₂ : clause} : c₁ ~ c₂ → clause.eval α c₁ = clause.eval α c₂ :=
+assume h, perm.foldr_eq (eval_op_left_comm α) h ff
+
+-- More set-like properties for evaluation
+theorem eval_tt_of_subset_eval_tt {α : assignment} {c₁ c₂ : clause} :
+  c₁ ⊆ c₂ → clause.eval α c₁ = tt → clause.eval α c₂ = tt :=
+begin
+  intros h₁ h₂,
+  apply eval_tt_iff_exists_literal_eval_tt.mpr,
+  rcases eval_tt_iff_exists_literal_eval_tt.mp h₂ with ⟨l, hl, he⟩,
+  use [l, h₁ hl, he]
+end
+
+theorem eval_ff_of_superset_eval_ff {α : assignment} {c₁ c₂ : clause} :
+  c₁ ⊆ c₂ → clause.eval α c₂ = ff → clause.eval α c₁ = ff :=
+begin
+  intros h₁ h₂,
+  apply eval_ff_iff_forall_literal_eval_ff.mpr,
+  intros l hl,
+  rw eval_ff_iff_forall_literal_eval_ff at h₂,
+  exact h₂ l (h₁ hl)
+end
+
+theorem eval_tt_of_sublist_eval_tt {α : assignment} {c₁ c₂ : clause} :
+  c₁ <+ c₂ → clause.eval α c₁ = tt → clause.eval α c₂ = tt :=
+assume h₁, eval_tt_of_subset_eval_tt (sublist.subset h₁)
+
+theorem eval_ff_of_superlist_eval_ff {α : assignment} {c₁ c₂ : clause} :
+  c₁ <+ c₂ → clause.eval α c₂ = ff → clause.eval α c₁ = ff :=
+assume h₁, eval_ff_of_superset_eval_ff (sublist.subset h₁)
+
+theorem eval_tt_cons_of_eval_tt {α : assignment} {c : clause} (l : literal) :
+  clause.eval α c = tt → clause.eval α (l :: c) = tt :=
+assume h, eval_tt_of_sublist_eval_tt (sublist_cons l c) h
+
+theorem eval_ff_of_eval_ff_cons {α : assignment} {c : clause} {l : literal} :
+  clause.eval α (l :: c) = ff → clause.eval α c = ff :=
+assume h, eval_ff_of_superlist_eval_ff (sublist_cons l c) h
+
+/-! # Falsify and truthify -/
 
 -- For any list of natural numbers and assignment, a false clause can be computed
 def falsify : assignment → list nat → clause
@@ -130,411 +196,196 @@ def truthify : assignment → list nat → clause
 @[simp] lemma falsify_nil (α : assignment) : falsify α [] = [] := rfl
 @[simp] lemma truthify_nil (α : assignment) : truthify α [] = [] := rfl
 
-theorem eval_ff_of_falsify (α : assignment) (ns : list nat) : eval α (falsify α ns) = ff :=
+theorem falsify_eval_ff (α : assignment) (l : list nat) : clause.eval α (falsify α l) = ff :=
 begin
-  induction ns with m ms ih,
-  { simp [falsify] },
-  { unfold falsify,
-    by_cases α m = tt,
-    { simp [h, eval_cons, literal.eval, ih] },
-    { simp at h,
-      simp [h, eval_cons, literal.eval, ih] } }
-end
-
-theorem eval_tt_of_truthify (α : assignment) {ns : list nat} (hns : ns ≠ []) : eval α (truthify α ns) = tt :=
-begin
-  induction ns with m ms ih,
-  { contradiction },
-  { by_cases α m = tt,
-    { simp [truthify, h, literal.eval, eval_cons] },
-    { simp at h, simp [truthify, h, literal.eval, eval_cons] } }
-end
-
-theorem map_var_falsify_eq_list (α : assignment) (ns : list nat) : map var (falsify α ns) = ns :=
-begin
-  induction ns with m ms ih,
+  induction l with n ns ih,
   { simp },
-  { rcases bool_by_cases (α m) with h | h;
+  { cases h : (α n);
+    { simp [falsify, h, eval_cons, literal.eval, ih] } }
+end
+
+theorem truthify_eval_tt (α : assignment) {l : list nat} (hl : l ≠ []) : 
+  clause.eval α (truthify α l) = tt :=
+begin
+  induction l with n ms ih,
+  { contradiction },
+  { cases h : (α n);
+    { simp [truthify, h, literal.eval, eval_cons] } }
+end
+
+-- Get rid of these next two?
+theorem map_var_falsify_eq_list (α : assignment) (l : list nat) : map var (falsify α l) = l :=
+begin
+  induction l with n ns ih,
+  { simp },
+  { cases h : (α n);
     { simp [falsify, h, ih, var] } }
 end
 
-theorem map_var_truthify_eq_list (α : assignment) (ns : list nat) : map var (truthify α ns) = ns :=
+theorem map_var_truthify_eq_list (α : assignment) (l : list nat) : map var (truthify α l) = l :=
 begin
-  induction ns with m ms ih,
+  induction l with n ns ih,
   { simp },
-  { rcases bool_by_cases (α m) with h | h;
+  { cases h : (α n);
     { simp [truthify, h, ih, var] } }
 end
 
-theorem flip_truthify_eq_falsify (α : assignment) (ns : list nat) :
-  map flip (truthify α ns) = falsify α ns :=
+theorem flip_truthify_eq_falsify (α : assignment) (l : list nat) : 
+  map flip (truthify α l) = falsify α l :=
 begin
-  induction ns with m ms ih,
-  { simp [truthify, falsify] },
-  { simp [truthify, falsify],
-    by_cases α m = tt,
-    { simp [h, literal.eval, ih, literal.flip] },
-    { simp at h, simp [h, literal.eval, ih, literal.flip] } }
-end
-
-theorem eval_erase_of_mem (α : assignment) {l : literal} {c : clause} (h : l ∈ c) : eval α c = (literal.eval α l) || (eval α (c.erase l)) :=
-begin
-  induction c with d ds ih,
-  { exact absurd h (not_mem_nil _) },
-  rcases classical.em (l = d) with rfl | hne,
-  { simp [erase_cons_head, eval_cons] },
-  { simp only [eval_cons, erase_cons_tail ds (ne.symm hne), ih (mem_of_ne_of_mem hne h), ← bool.bor_assoc, bool.bor_comm] }
-end
-
-theorem eval_erase_of_not_mem {α : assignment} {l : literal} {c : clause} (h : l ∉ c) : eval α c = eval α (c.erase l) :=
-by simp [erase_of_not_mem h]
-
-/-! ### Similarity of clauses -/
--- Because clauses are literals joined by ORs, and OR is commutative, similar clauses evaluate identically
-
-theorem eval_sim (α : assignment) {c₁ : clause} : ∀ (c₂ : clause), c₁ ~ c₂ → eval α c₁ = eval α c₂ :=
-begin
-  induction c₁ with l c ih; intros c₂ h,
-  { simp [perm.nil_eq h] },
-  { simp only [ih (c₂.erase l) (cons_perm_iff_perm_erase.mp h).2, 
-      eval_cons, (eval_erase_of_mem α ((perm.mem_iff h).mp (mem_cons_self l c))).symm] }
-end
-
--- A potentially helpful lemma stating that if a clause mapped to vars is similar to a list,
--- then for any nat, there is a literal whose variable is that nat
--- NOTE: Another version of this can be proven with no duplicates in either the clause or the list, via ↔
-lemma all_mem_of_sim_var {ns : list nat} : ∀ (c : clause), c.map var ~ ns → ∀ n ∈ ns, ∃ l ∈ c, literal.var l = n :=
-begin
-  intros c hsim n hn,
-  rcases exists_of_mem_map ((perm.mem_iff hsim).mpr hn) with ⟨a, ⟨ha1, ha2⟩⟩,
-  use a, exact and.intro ha1 ha2
-end
-
--- TODO cleanup with split and cases
-lemma erase_map_var_eq_map_var_erase {c : clause} : 
-  ∀ (n : nat), n ∈ c.map var → ∃ (l : literal), l ∈ c ∧ l.var = n ∧ (c.map var).erase n ~ (c.erase l).map var :=
-begin
-  induction c with l ls ih; intros n hn,
-  { rw map_nil at hn, exact absurd hn (not_mem_nil _) },
-  by_cases l.var = n,
-  { use l, split, { exact mem_cons_self l ls },
-    split, { exact h },
-    simp only [mem_cons_self, erase_cons_head, map_cons, h, perm.refl] },
-  rcases mem_map.mp hn with ⟨a, ⟨hal, han⟩⟩,
-  have hcase := h,
-  rw ← han at h,
-  have laneq : l ≠ a, from ne_of_apply_ne (λ (l : literal), l.var) h,
-  have hals : a ∈ ls, from mem_of_ne_of_mem laneq.symm hal,
-  have hamap : a.var ∈ map var ls, from mem_map_of_mem var hals,
-  rw han at hamap,
-  have ihred := ih n hamap,
-  rcases ihred with ⟨l2, ⟨hl2ls, ⟨hl2n, hl2sim⟩⟩⟩,
-  use l2,
-  have hl2lls : l2 ∈ l :: ls, from mem_cons_of_mem l hl2ls,
-  by_cases l2 = l,
-  { rw h at hl2n, exact absurd hl2n hcase },
-  rw erase_cons_tail ls (ne.symm h),
-  rw map_cons,
-  rw map_cons,
-  rw erase_cons_tail (map var ls) hcase,
-  exact and.intro hl2lls (and.intro (hl2n) (perm.cons l.var hl2sim))
-end
-
-theorem map_var_sim_of_var_of_mem {n : nat} {l : literal} {c : clause} : 
-  l ∈ c → l.var = n → (map var c).erase n ~ map var (c.erase l) :=
-begin
-  induction c with d ds ih,
-  { intro h, exact absurd h (not_mem_nil _) },
-  { intros hds hn,
-    by_cases l = d,
-    { rw h at hn, simp [erase_cons, h, hn] },
-    { have : l ∈ ds, from mem_of_ne_of_mem h hds,
-      have ihred := ih (mem_of_ne_of_mem h hds) hn,
-      simp [ihred, erase_cons, (ne.symm h)],
-      by_cases (d.var = l.var),
-      { simp [h, hn],
-        have : var l ∈ map var ds, from mem_map_of_mem var this,
-        rw hn at this,
-        exact perm.trans (perm_cons_erase this) (perm.cons n ihred) },
-      { simp [ne_of_ne_of_eq h hn, ihred] } } }
+  induction l with n ns ih,
+  { simp },
+  { cases h : (α n);
+    { simp [h, literal.eval, ih, literal.flip, truthify, falsify] } }
 end
 
 /-! ### Counting -/
+
 /- Counts the number of literals that evaluate to true in the clause, under some assignment -/
 def count_tt (α : assignment) (c : clause) : nat :=
-  c.countp (λ l, l.eval α = tt)
+  c.countp (λ l, literal.eval α l = tt)
 
 /- Counts the number of literals that evaluate to false in the clause, under some assignment -/
 def count_ff (α : assignment) (c : clause) : nat :=
-  c.countp (λ l, l.eval α = ff)
+  c.countp (λ l, literal.eval α l = ff)
 
 /- Counts the number of positive literals in the clause -/
 def count_pos (c : clause) : nat :=
-  c.countp (λ l, literal.is_pos l = tt)
+  c.countp (λ l, is_pos l = tt)
 
 /- Counts the number of negative literals in the clause -/
 def count_neg (c : clause) : nat :=
-  c.countp (λ l, literal.is_neg l = tt)
+  c.countp (λ l, is_neg l = tt)
 
 @[simp] lemma count_tt_nil (α : assignment) : count_tt α [] = 0 := by dec_trivial
 @[simp] lemma count_ff_nil (α : assignment) : count_ff α [] = 0 := by dec_trivial
 @[simp] lemma count_pos_nil : count_pos [] = 0 := by dec_trivial
 @[simp] lemma count_neg_nil : count_neg [] = 0 := by dec_trivial
 
-lemma count_tt_cons (α : assignment) (l : literal) (c : clause) : count_tt α (l :: c) = bool.to_nat (l.eval α) + count_tt α c :=
-begin
-  unfold count_tt, cases classical.em (l.eval α = tt),
-  { simp [countp_cons_of_pos (λ l, literal.eval α l = tt) c h, h, bool.to_nat, add_comm] },
-  { simp [countp_cons_of_neg (λ l, literal.eval α l = tt) c h, h, bool.to_nat, bool_eq_false h] }
-end
+@[simp] theorem count_tt_singleton (α : assignment) (l : literal) : 
+  count_tt α [l] = bool.to_nat (literal.eval α l) :=
+by cases h : (literal.eval α l); { simp [h, count_tt, bool.to_nat] }
 
-lemma count_ff_cons (α : assignment) (l : literal) (c : clause) : count_ff α (l :: c) = bool.to_nat (!l.eval α) + count_ff α c :=
-begin
-  unfold count_ff, cases classical.em (l.eval α = ff),
-  { simp [countp_cons_of_pos (λ l, literal.eval α l = ff) c h, h, bool.to_nat, add_comm] },
-  { simp [countp_cons_of_neg (λ l, literal.eval α l = ff) c h, bool.to_nat, eq_tt_of_not_eq_ff h] }
-end
+@[simp] theorem count_ff_singleton (α : assignment) (l : literal) :
+  count_ff α [l] = bool.to_nat (!literal.eval α l) :=
+by cases h : (literal.eval α l); { simp [h, count_ff, bool.to_nat] }
 
-lemma count_pos_cons (l : literal) (c : clause) : count_pos (l :: c) = bool.to_nat (l.is_pos) + count_pos c :=
-begin
-  unfold count_pos, cases classical.em (l.is_pos = tt),
-  { simp [countp_cons_of_pos (λ l, literal.is_pos l = tt) c h, h, bool.to_nat, add_comm] },
-  { simp [countp_cons_of_neg (λ l, literal.is_pos l = tt) c h, bool.to_nat, bool_eq_false h] }
-end
+@[simp] theorem count_pos_singleton (l : literal) : 
+  count_pos [l] = bool.to_nat (is_pos l) :=
+by cases l; simp [count_pos, bool.to_nat, countp, is_pos]
 
-lemma count_neg_cons (l : literal) (c : clause) : count_neg (l :: c) = bool.to_nat (l.is_neg) + count_neg c :=
-begin
-  unfold count_neg, cases classical.em (l.is_neg = tt),
-  { simp [countp_cons_of_pos (λ l, literal.is_neg l = tt) c h, h, bool.to_nat, add_comm] },
-  { simp [countp_cons_of_neg (λ l, literal.is_neg l = tt) c h, bool.to_nat, bool_eq_false h] }
-end
+@[simp] theorem count_neg_singleton (l : literal) : 
+  count_neg [l] = bool.to_nat (is_neg l) :=
+by cases l; simp [count_neg, bool.to_nat, countp, is_neg]
 
-lemma count_tt_singleton (α : assignment) (l : literal) : count_tt α [l] = bool.to_nat (l.eval α) := by simp [count_tt_cons α l []]
-lemma count_ff_singleton (α : assignment) (l : literal) : count_ff α [l] = bool.to_nat (!l.eval α) := by simp [count_ff_cons α l []]
-lemma count_pos_singleton (l : literal) : count_pos [l] = bool.to_nat l.is_pos := by simp [count_pos_cons l []]
-lemma count_neg_singleton (l : literal) : count_neg [l] = bool.to_nat l.is_neg := by simp [count_neg_cons l []]
+theorem count_tt_cons (α : assignment) (l : literal) (c : clause) : 
+  count_tt α (l :: c) = bool.to_nat (literal.eval α l) + count_tt α c :=
+by cases h : (literal.eval α l); { simp [h, bool.to_nat, and_comm, add_comm, count_tt] }
 
-lemma count_tt_falsify (α : assignment) (c : clause) : count_tt α (falsify α (map var c)) = 0 :=
+theorem count_ff_cons (α : assignment) (l : literal) (c : clause) : 
+  count_ff α (l :: c) = bool.to_nat (!literal.eval α l) + count_ff α c :=
+by cases h : (literal.eval α l); { simp [h, bool.to_nat, and_comm, add_comm, count_ff] }
+
+theorem count_pos_cons (l : literal) (c : clause) : 
+  count_pos (l :: c) = bool.to_nat (is_pos l) + count_pos c :=
+by cases h : (is_pos l); { simp [h, bool.to_nat, add_comm, count_pos] }
+
+theorem count_neg_cons (l : literal) (c : clause) : 
+  count_neg (l :: c) = bool.to_nat (is_neg l) + count_neg c :=
+by cases h : (is_neg l); { simp [h, bool.to_nat, add_comm, count_neg] }
+
+-- All the above four functions are capped by the length of the clause
+theorem count_tt_le_length (α : assignment) (c : clause) : count_tt α c ≤ length c :=
+by simp only [count_tt, countp_eq_length_filter, length_filter]
+
+theorem count_ff_le_length (α : assignment) (c : clause) : count_ff α c ≤ length c :=
+by simp only [count_ff, countp_eq_length_filter, length_filter]
+
+theorem count_pos_le_length (c : clause) : count_pos c ≤ length c :=
+by simp only [count_pos, countp_eq_length_filter, length_filter]
+
+theorem count_neg_le_length (c : clause) : count_neg c ≤ length c :=
+by simp only [count_neg, countp_eq_length_filter, length_filter]
+
+-- count_tt and count_ff are complements of each other
+-- There's probably an astute nat lemma that cleans this up
+theorem count_tt_eq_length_sub_cont_ff (α : assignment) (c : clause) :
+  count_tt α c = length c - count_ff α c :=
 begin
   induction c with l ls ih,
   { simp },
-  { rcases exists_nat_of_lit l with ⟨n, (rfl | rfl)⟩;
-    { rcases bool_by_cases (α n) with h | h;
-      { simp [falsify, h, var, count_tt_cons, bool.to_nat, literal.eval, ih] } } }
+  { cases h : (literal.eval α l);
+    simp [count_tt_cons, count_ff_cons, h, bool.to_nat, ih, add_comm 1, nat.add_sub_add_right],
+    { rw add_comm ls.length 1,
+      rw nat.add_sub_assoc (count_ff_le_length α ls) 1,
+      rw add_comm } }
 end
+
+-- count_pos and count_neg are complements of each other
+theorem count_pos_eq_length_sub_count_neg (c : clause) :
+  count_pos c = length c - count_neg c :=
+begin
+  induction c with l ls ih,
+  { simp },
+  { cases l;
+    simp [ih, count_pos_cons, count_neg_cons, bool.to_nat, is_pos, is_neg],
+    { rw add_comm ls.length 1,
+      rw nat.add_sub_assoc (count_neg_le_length ls) 1 },
+    { simp [add_comm 1] } }
+end
+
+lemma count_tt_eq_zero_of_eval_ff {α : assignment} {c : clause} :
+  clause.eval α c = ff → count_tt α c = 0 :=
+begin
+  induction c with l ls ih,
+  { simp },
+  { simp [eval_cons, count_tt_cons],
+    intros hl hls,
+    simp [hl, bool.to_nat, ih hls] }
+end
+
+lemma eval_ff_of_count_tt_eq_zero {α : assignment} {c : clause} :
+  count_tt α c = 0 → clause.eval α c = ff :=
+begin
+  induction c with l ls ih,
+  { simp },
+  { simp [eval_cons, count_tt_cons, bool.to_nat, literal.eval],
+    intros hl hls,
+    simp [cond_ff_of_cond_eq_second_of_ne _ one_ne_zero hl, ih hls] }
+end
+
+theorem count_tt_eq_zero_iff_eval_ff {α : assignment} {c : clause} :
+  clause.eval α c = ff ↔ count_tt α c = 0 :=
+⟨count_tt_eq_zero_of_eval_ff, eval_ff_of_count_tt_eq_zero⟩
+
+lemma count_tt_gt_zero_of_eval_tt {α : assignment} {c : clause} :
+  clause.eval α c = tt → count_tt α c > 0 :=
+begin
+  induction c with l ls ih,
+  { simp },
+  { cases h : (literal.eval α l);
+    simp [h, eval_cons, count_tt_cons, bool.to_nat],
+    { intro hls, exact ih hls },
+    { exact nat.zero_lt_one_add _ } }
+end
+
+lemma eval_tt_of_count_tt_gt_zero {α : assignment} {c : clause} :
+  0 < count_tt α c → clause.eval α c = tt :=
+by { simp only [count_tt, countp_pos, eval_tt_iff_exists_literal_eval_tt], exact id }
+
+theorem count_tt_gt_zero_iff_eval_tt {α : assignment} {c : clause} :
+  clause.eval α c = tt ↔ count_tt α c > 0 :=
+⟨count_tt_gt_zero_of_eval_tt, eval_tt_of_count_tt_gt_zero⟩
+
+theorem count_tt_falsify (α : assignment) (l : list nat) : count_tt α (falsify α l) = 0 :=
+count_tt_eq_zero_iff_eval_ff.mp (falsify_eval_ff α l)
 
 lemma count_tt_truthify (α : assignment) (c : clause) : count_tt α (truthify α (map var c)) = length c :=
 begin
   induction c with l ls ih,
   { simp },
-  { rcases exists_nat_of_lit l with ⟨n, (rfl | rfl)⟩;
-  { rcases bool_by_cases (α n) with h | h;
+  { cases l; { cases h : (α l);
     { simp [truthify, h, var, count_tt_cons, bool.to_nat, literal.eval, ih, add_comm] } } }
-end
-
-lemma count_pos_subset {c₁ c₂ : clause} : c₁ <+ c₂ → count_pos c₁ ≤ count_pos c₂ := 
-  assume h, by simp [count_pos, countp_le_of_sublist (λ l, literal.is_pos l = tt) h]
-
-lemma count_neg_subset {c₁ c₂ : clause} : c₁ <+ c₂ → count_neg c₁ ≤ count_neg c₂ :=
-  assume h, by simp [count_neg, countp_le_of_sublist (λ l, literal.is_neg l = tt) h]
-
-lemma exists_pos_of_odd_count_pos {c : clause} : c.count_pos.bodd → ∃ (n : nat), Pos n ∈ c :=
-begin
-  induction c with cl cls ih, --; intro h,
-  { simp [nat.bodd_zero] },
-  { intro h,
-    rcases exists_nat_of_lit cl with ⟨n, (rfl | rfl)⟩,
-    { use n, exact mem_cons_self (Pos n) cls },
-    { simp [count_pos_cons, is_pos, bool.to_nat] at h,
-      rcases ih h with ⟨n2, h2⟩, use n2, simp [h2] } }
-end
-
-lemma count_tt_le_length (α : assignment) (c : clause) : count_tt α c ≤ length c :=
-by simp [count_tt, countp_eq_length_filter, length_filter]
-
--- Handling the erase case
-lemma count_pos_erase_of_mem {c : clause} {l : literal} (h : l ∈ c) : count_pos c = count_pos (c.erase l) + count_pos [l] :=
-begin
-  induction c with d ds ih,
-  { exact absurd h ( not_mem_nil _) },
-  rcases eq_or_ne_mem_of_mem h with rfl | ⟨hne, h2⟩,
-  { simp [erase_cons_head, count_pos_cons, add_comm] },
-  { rw erase_cons_tail ds (ne.symm hne),
-    have : count_pos [l] ≤ count_pos ds, from count_pos_subset (singleton_sublist.mpr h2),
-    simp [count_pos_singleton] at this,
-    simp [count_pos_cons, ih h2, add_assoc] }
-end
-
-lemma count_neg_erase_of_mem {c : clause} {l : literal} (h : l ∈ c) : count_neg c = count_neg (c.erase l) + count_neg [l] :=
-begin
-  induction c with d ds ih,
-  { exact absurd h ( not_mem_nil _) },
-  rcases eq_or_ne_mem_of_mem h with rfl | ⟨hne, h2⟩,
-  { simp [erase_cons_head, count_neg_cons, add_comm] },
-  { rw erase_cons_tail ds (ne.symm hne),
-    have : count_neg [l] ≤ count_neg ds, from count_neg_subset (singleton_sublist.mpr h2),
-    simp [count_neg_singleton] at this,
-    simp [count_neg_cons, ih h2, add_assoc] }
-end
-
-theorem exists_literal_eval_tt_of_pos_count_tt {α : assignment} {c : clause} : 
-  0 < count_tt α c → ∃ (l : literal), l ∈ c ∧ l.eval α = tt :=
-begin
-  induction c with l ls ih,
-  { simp [count_tt] },
-  { rcases bool_by_cases (l.eval α),
-    { intro _, use l, simp [h, mem_cons_self l ls] },
-    { simp [count_tt_cons, h, bool.to_nat],
-      intro hls,
-      rcases ih hls with ⟨m, hm⟩,
-      use m,
-      simp [hm] } }
-end
-
--- Corollary of the above by definition of clause evaluation
-theorem eval_tt_of_pos_count_tt {α : assignment} {c : clause} :
-  0 < count_tt α c → eval α c = tt :=
-begin
-  intro h,
-  apply eval_tt_iff_exists_literal_tt.mpr,
-  simp [exists_literal_eval_tt_of_pos_count_tt h]
-end
-
-theorem forall_literal_eval_ff_of_count_tt_eq_zero {α : assignment} {c : clause} :
-  count_tt α c = 0 → ∀ {l : literal}, l ∈ c → l.eval α = ff :=
-begin
-  induction c with l ls ih,
-  { simp },
-  { intros h m hm,
-    simp [count_tt_cons, bool.to_nat] at h,
-    rcases h with ⟨hcond, hls⟩,
-    rcases eq_or_ne_mem_of_mem hm with (hlm | ⟨_, hin⟩),
-    { simp [hlm, cond_ff_of_cond_eq_second_of_ne (ne.symm zero_ne_one) hcond] },
-    { exact ih hls hin } }
-end
-
-theorem eval_ff_of_count_tt_eq_zero {α : assignment} {c : clause} :
-  count_tt α c = 0 → eval α c = ff :=
-begin
-  intro h,
-  apply eval_ff_iff_literals_ff.mpr,
-  intros _ hl,
-  exact forall_literal_eval_ff_of_count_tt_eq_zero h hl
-end
-
--- Flip counting
-def count_flips : clause → clause → nat
-| []         _        := 0
-| _         []        := 0
-| (l :: ls) (m :: ms) := ite (l.flip = m) (1 + count_flips ls ms) (count_flips ls ms)
-
-@[simp] lemma count_flips_nil (c₁ c₂ : clause) : c₁ = [] ∨ c₂ = [] → count_flips c₁ c₂ = 0 :=
-begin
-  intro h, rcases h with rfl | rfl, 
-  { rcases list_by_cases c₂ with rfl | ⟨b, L, rfl⟩;
-    { simp [count_flips] } },
-  { rcases list_by_cases c₁ with rfl | ⟨b, L, rfl⟩;
-    { simp [count_flips] } }
-end
-
-lemma count_flips_self (c : clause) : count_flips c c = 0 :=
-begin
-  induction c with l ls ih,
-  { simp },
-  { simp [count_flips, ne_flip_self, ih] }
-end
-
-lemma count_flips_comm (c₁ : clause) : ∀ (c₂ : clause), count_flips c₁ c₂ = count_flips c₂ c₁ :=
-begin
-  induction c₁ with l ls ih,
-  { simp },
-  { intro c₂,
-    rcases list_by_cases c₂ with rfl | ⟨m, ms, rfl⟩,
-    { simp [count_flips] },
-    { simp [count_flips],
-      by_cases l.flip = m,
-      { simp [h, eq_flip_of_flip_eq h, eq_flip_flip, ih] },
-      { simp [h, ne.symm (ne_flip_of_flip_ne h), eq_flip_flip, ih] } } }
-end
-
-theorem count_flips_pos_of_neq_of_map_var_eq {c₁ : clause} :
-  ∀ {c₂ : clause}, map var c₁ = map var c₂ → c₁ ≠ c₂ → count_flips c₁ c₂ > 0 :=
-begin
-  induction c₁ with l ls ih,
-  { intros c₂ h,
-    simp at h,
-    rw eq_nil_of_map_eq_nil h.symm,
-    contradiction },
-  { intros c₂ h hneq,
-    rcases exists_cons_of_map_cons h.symm with ⟨x, xs, rfl, hxl, hxs⟩,
-    by_cases heq : l = x,
-    { simp [count_flips, ih hxs.symm (ne_tail_of_eq_head_of_ne hneq heq), heq, ne_flip_self] },
-    { simp [count_flips, eq_flip_of_eq_var_of_ne heq hxl.symm, nat.zero_lt_one_add] } }
-end
-
-theorem count_flips_falsify_eq_count_tt (α : assignment) (c : clause) :
-  count_flips c (falsify α (map var c)) = count_tt α c :=
-begin
-  induction c with l ls ih,
-  { simp },
-  { rcases exists_nat_of_lit l with ⟨n, (rfl | rfl)⟩;
-    { rcases bool_by_cases (α n) with h | h;
-      { simp [falsify, count_flips, h, var, literal.flip, 
-              count_tt_cons, ih, bool.to_nat, literal.eval] } } }
-end
-
-/-! ## Parity reasoning for evaluation -/
-
--- This can probably be vastly shortened with a restatement or the introduction with a few supporting lemmas
-theorem eval_tt_of_neq_counts {α : assignment} {ns : list nat} (hnil : ns ≠ nil) (hns : ns.nodup) :
-  ∀ (c : clause), map var c = ns → count_tt α (map Pos ns) ≠ count_neg c → eval α c = tt :=
-begin
-  induction ns with m ms ih,
-  { contradiction },
-  by_cases ms = nil,
-  { rw h,
-    intros c hc hcount,
-    rcases exists_of_map_singleton hc with ⟨l, rfl, hl⟩,
-    rcases pos_or_neg_of_var_eq_nat hl with rfl | rfl,
-    { simp [literal.eval],
-      by_cases α m = tt,
-      { exact h },
-      { simp at h,
-        simp [count_tt_singleton, count_neg_singleton, is_neg, bool.to_nat, h, literal.eval] at hcount,
-        exfalso, exact hcount } },
-    { simp [literal.eval],
-      by_cases α m = tt,
-      { simp [count_tt_singleton, count_neg_singleton, is_neg, bool.to_nat, h, literal.eval] at hcount, 
-        exfalso, exact hcount },
-      { simp at h, exact h } } },
-  { intros c hc hcount,
-    rcases exists_cons_of_map_cons hc with ⟨l, ls, rfl, hl, hls⟩,
-    have ihred := ih h (nodup_of_nodup_cons hns) ls hls,
-    rw eval_cons,
-    by_cases literal.eval α l = tt,
-    { simp [h] },
-    { simp at h,
-      rcases pos_or_neg_of_var_eq_nat hl with rfl | rfl,
-      { simp [h],
-        simp [count_tt_cons, count_neg_cons, h, bool.to_nat, is_neg] at hcount,
-        exact ihred hcount },
-      { simp [count_tt_cons, count_neg_cons, h, bool.to_nat, is_neg] at hcount,
-        have : literal.eval α (Pos m) = tt, 
-        { have h3 := literal.eval_flip α (Pos m),
-          simp [literal.flip] at h3,
-          rw h at h3,
-          simp at h3,
-          exact h3 },
-        simp [this] at hcount,
-        simp [ihred hcount] } } }
-end
-
--- Corollary of the above wrt parity reasoning
-theorem eval_tt_of_opposite_parity {α : assignment} {ns : list nat} {c : clause} (hnil : ns ≠ nil) (hns : ns.nodup) : 
-  map var c = ns → nat.bodd (count_tt α (map Pos ns)) ≠ nat.bodd (count_neg c) → eval α c = tt :=
-begin
-  intros hc hcount,
-  exact eval_tt_of_neq_counts hnil hns c hc (ne_of_apply_ne nat.bodd hcount)
 end
 
 -- Falsify negates those literals that, if positive, are true
@@ -543,73 +394,322 @@ theorem count_tt_pos_eq_count_neg_falsify (α : assignment) (ns : list nat) :
 begin
   induction ns with m ms ih,
   { simp },
-  { rcases bool_by_cases (α m) with h | h;
+  { cases h : (α m);
     { simp [count_tt_cons, h, falsify, count_neg_cons, literal.eval, is_neg, bool.to_nat, ih] } }
 end
+
+-- Sublist theorems (can have subset theorems too)
+theorem count_pos_sublist {c₁ c₂ : clause} : c₁ <+ c₂ → count_pos c₁ ≤ count_pos c₂ := 
+assume h, by simp [count_pos, countp_le_of_sublist (λ l, is_pos l = tt) h]
+
+theorem count_neg_sublist {c₁ c₂ : clause} : c₁ <+ c₂ → count_neg c₁ ≤ count_neg c₂ :=
+assume h, by simp [count_neg, countp_le_of_sublist (λ l, is_neg l = tt) h]
+
+theorem count_tt_sublist (α : assignment) {c₁ c₂ : clause} : c₁ <+ c₂ → count_tt α c₁ ≤ count_tt α c₂ :=
+assume h, by simp [count_tt, countp_le_of_sublist (λ l, literal.eval α l = tt) h]
+
+theorem count_ff_sublist (α : assignment) {c₁ c₂ : clause} : c₁ <+ c₂ → count_ff α c₁ ≤ count_ff α c₂ :=
+assume h, by simp [count_ff, countp_le_of_sublist (λ l, literal.eval α l = ff) h]
+
+theorem exists_pos_iff_pos_count_pos {c : clause} : count_pos c > 0 ↔ ∃ l ∈ c, is_pos l :=
+by simp [count_pos, countp_pos]
+
+theorem exists_neg_iff_pos_count_neg {c : clause} : count_neg c > 0 ↔ ∃ l ∈ c, is_neg l :=
+by simp [count_neg, countp_pos]
+
+theorem exists_tt_iff_pos_count_tt {α : assignment} {c : clause} : count_tt α c > 0 ↔ ∃ l ∈ c, literal.eval α l = tt :=
+by simp [count_tt, countp_pos]
+
+theorem exists_ff_iff_pos_count_ff {α : assignment} {c : clause} : count_ff α c > 0 ↔ ∃ l ∈ c, literal.eval α l = ff :=
+by simp [count_ff, countp_pos]
+
+/-! # Flip counting -/
+
+-- Flip counting
+-- Not good from a set perspective, as order must be maintained
+def count_flips : clause → clause → nat
+| []         _        := 0
+| _         []        := 0
+| (l :: ls) (m :: ms) := ite (l.flip = m) (1 + count_flips ls ms) (count_flips ls ms)
+
+@[simp] lemma count_flips_nil (c₁ c₂ : clause) : c₁ = [] ∨ c₂ = [] → count_flips c₁ c₂ = 0 :=
+begin
+  intro h, rcases h with rfl | rfl, 
+  { cases c₂; { simp [count_flips] } },
+  { cases c₁; { simp [count_flips] } }
+end
+
+theorem count_flips_cons (c₁ c₂ : clause) (l₁ l₂ : literal) :
+  count_flips (l₁ :: c₁) (l₂ :: c₂) = bool.to_nat (l₁.flip = l₂) + count_flips c₁ c₂ :=
+by { by_cases l₁.flip = l₂; simp [count_flips, h, bool.to_nat] }
+
+lemma count_flips_self (c : clause) : count_flips c c = 0 :=
+begin
+  induction c with l ls ih,
+  { simp },
+  { simp [count_flips, flip_ne, ih] }
+end
+
+lemma count_flips_comm (c₁ : clause) : ∀ (c₂ : clause), count_flips c₁ c₂ = count_flips c₂ c₁ :=
+begin
+  induction c₁ with l ls ih,
+  { simp },
+  { intro c₂, cases c₂,
+    { simp [count_flips] },
+    { simp [count_flips, ih c₂_tl],
+      cases classical.em (l.flip = c₂_hd),
+      { simp [h, (congr_arg literal.flip h).symm], rw flip_flip l, simp },
+      { have : l.flip.flip ≠ c₂_hd.flip, from flip_injective.ne h,
+        rw flip_flip at this,
+        simp [h, (ne.symm this)] } } }
+end
+
+theorem count_flips_pos_of_neq_of_map_var_eq {c₁ : clause} :
+  ∀ {c₂ : clause}, map var c₁ = map var c₂ → c₁ ≠ c₂ → count_flips c₁ c₂ > 0 :=
+begin
+  induction c₁ with l ls ih,
+  { intros c₂ h,
+    simp at h,
+    simp [eq_nil_of_map_eq_nil h.symm] },
+  { intros c₂ h hneq,
+    rcases exists_cons_of_map_cons h.symm with ⟨x, xs, rfl, hxl, hxs⟩,
+    by_cases heq : l = x,
+    { simp [count_flips, ih hxs.symm (ne_tail_of_eq_head_of_ne hneq heq), heq, flip_ne] },
+    { rcases eq_or_flip_eq_of_var_eq hxl.symm with rfl | hlf,
+      { contradiction },
+      { simp [count_flips, nat.zero_lt_one_add, hlf] } } }
+end
+
+theorem count_flips_falsify_eq_count_tt (α : assignment) (c : clause) :
+  count_flips c (falsify α (map var c)) = count_tt α c :=
+begin
+  induction c with l ls ih,
+  { simp },
+  { cases l; { cases h : (α l);
+    { simp [falsify, count_flips, h, var, literal.flip, count_tt_cons, bool.to_nat, literal.eval, ih] } } }
+end
+
+/-! ## Parity reasoning for evaluation -/
+
+-- This can probably be vastly shortened with a restatement or the introduction with a few supporting lemmas
+theorem eval_tt_of_neq_counts {α : assignment} {ns : list nat} (hnil : ns ≠ []) :
+  ∀ (c : clause), map var c = ns → count_tt α (map Pos ns) ≠ count_neg c → clause.eval α c = tt :=
+begin
+  induction ns with m ms ih,
+  { contradiction },
+  { cases ms,
+    { intros c hc hne,
+      rcases exists_of_map_singleton hc with ⟨l, rfl, hl⟩,
+      cases l; simp [is_neg, bool.to_nat] at hne; simp only [var] at hl,
+      { simp [hl, cond_tt_of_not_cond_eq_second_of_ne (literal.eval α (Pos m)) one_ne_zero hne] },
+      { have := cond_ff_of_not_cond_eq_first_of_ne (literal.eval α (Pos m)) zero_ne_one hne,
+        simp [literal.eval] at this,
+        simp [this, literal.eval, hl] } },
+    { intros c hc hcount,
+      rcases exists_cons_of_map_cons hc with ⟨l, ls, rfl, hl, hls⟩,
+      have ihred := ih (cons_ne_nil ms_hd ms_tl) ls hls,
+      cases l; rw var at hl,
+      { cases h : (α m),
+        { rw [map_cons, count_tt_cons] at hcount,
+          simp only [count_neg_cons, literal.eval, h, is_neg, bool.to_nat, cond, zero_add] at hcount,
+          exact eval_tt_cons_of_eval_tt (Pos l) (ihred hcount) },
+        { simp [eval_cons, literal.eval, h, hl] } },
+      { cases h : (α m),
+        { simp [eval_cons, literal.eval, h, hl] },
+        { rw [map_cons, count_tt_cons] at hcount,
+          simp only [count_neg_cons, literal.eval, h, is_neg, bool.to_nat, cond] at hcount,
+          exact eval_tt_cons_of_eval_tt (Neg l) (ihred (ne_of_apply_ne (has_add.add 1) hcount)) } } } }
+end
+
+-- Basically the same proof here - shorten the above one, shorten this one
+-- Take complement of the ≠ statement with length c to get the premises of the above?
+theorem eval_tt_of_neq_counts2 {α : assignment} {ns : list nat} (hnil : ns ≠ []) :
+  ∀ (c : clause), map var c = ns → count_ff α (map Pos ns) ≠ count_pos c → clause.eval α c = tt :=
+begin
+  induction ns with m ms ih,
+  { contradiction },
+  { cases ms;
+    intros c hc hne,
+    { rcases exists_of_map_singleton hc with ⟨l, rfl, hl⟩,
+      cases l; simp [is_pos, bool.to_nat] at hne; simp only [var] at hl,
+      { have := cond_ff_of_not_cond_eq_first_of_ne (literal.eval α (Neg m)) zero_ne_one hne,
+        simp [literal.eval] at this,
+        simp [hl, this, literal.eval] },
+      { have := cond_tt_of_not_cond_eq_second_of_ne (!literal.eval α (Pos m)) one_ne_zero hne,
+        simp [literal.eval] at this,
+        simp [this, literal.eval, hl] } },
+    { rcases exists_cons_of_map_cons hc with ⟨l, ls, rfl, hl, hls⟩,
+      have ihred := ih (cons_ne_nil ms_hd ms_tl) ls hls,
+      cases l; rw var at hl,
+      { cases h : (α m),
+        { rw [map_cons, count_ff_cons] at hne,
+          simp only [count_pos_cons, literal.eval, h, is_pos, bool.to_nat, cond, bnot] at hne,
+          exact eval_tt_cons_of_eval_tt (Pos l) (ihred (ne_of_apply_ne (has_add.add 1) hne)) },
+        { simp [eval_cons, literal.eval, h, hl] } },
+      { cases h : (α m),
+        { simp [eval_cons, literal.eval, h, hl] },
+        { rw [map_cons, count_ff_cons] at hne,
+          simp only [count_neg_cons, literal.eval, h, is_pos, bool.to_nat, cond, bnot, zero_add] at hne,
+          exact eval_tt_cons_of_eval_tt (Neg l) (ihred hne) } } } }
+end
+
+-- Corollary of the above wrt parity reasoning
+theorem eval_tt_of_opposite_parity {α : assignment} {ns : list nat} {c : clause} (hnil : ns ≠ nil) : 
+  map var c = ns → nat.bodd (count_tt α (map Pos ns)) ≠ nat.bodd (count_neg c) → clause.eval α c = tt :=
+assume hc hcount, eval_tt_of_neq_counts hnil c hc (ne_of_apply_ne nat.bodd hcount)
 
 -- Parity reasoning based on flips rather than negs
 -- If a clause evaluates to false, then any clause that can be made by flipping a
 -- variable in that clause will evaluate to true
--- TODO clean up, especially instances of "this"
-theorem eval_tt_of_neq_flips {α : assignment} {c₁ : clause} (hc₁ : c₁ ≠ []) (hnodup : (map var c₁).nodup) :
-  ∀ (c₂ : clause), map var c₁ = map var c₂ → count_tt α c₁ ≠ count_flips c₁ c₂ → eval α c₂ = tt :=
+-- Shorten without much cases? Develop new tactic for symmetric casework?
+theorem eval_tt_of_neq_flips {α : assignment} {c₁ : clause} (hc₁ : c₁ ≠ []) :
+  ∀ (c₂ : clause), map var c₁ = map var c₂ → count_tt α c₁ ≠ count_flips c₁ c₂ → clause.eval α c₂ = tt :=
 begin
   induction c₁ with l ls ih,
   { contradiction },
-  { intros c₂ hmap hne,
-    rcases list_by_cases ls with rfl | ⟨m, ms, rfl⟩,
-    { simp at hmap,
-      rcases exists_of_map_singleton hmap.symm with ⟨m, rfl, hm⟩,
-      by_cases hmeq : m = l,
-      { simp [count_flips, hmeq, ne_flip_self] at hne,
-        simp [eval_tt_of_pos_count_tt (pos_iff_ne_zero.mpr hne), hmeq] },
-      { simp [count_flips, hmeq, eq_flip_of_eq_var_of_ne (ne.symm hmeq) hm.symm] at hne,
-        have := count_tt_le_length α [l],
-        simp at this,
-        have : count_tt α [l] = 0, from nat.lt_one_iff.mp ((ne.le_iff_lt hne).mp this),
-        have eval_ff := forall_literal_eval_ff_of_count_tt_eq_zero this (mem_singleton_self l),
-        rw (eq_flip_of_eq_var_of_ne (ne.symm hmeq) hm.symm).symm,
-        have := eval_flip α l,
-        rw eval_ff at this,
-        simp [bool.eq_tt_of_bnot_eq_ff this.symm] } },
-    { rw map_cons at hnodup,
-      rcases exists_map_cons_of_map_cons hmap.symm with ⟨n, ns, rfl, hn, hns⟩,
-      have ihred := ih (cons_ne_nil m ms) (nodup_cons.mp hnodup).2 ns hns.symm,
-      rcases bool_by_cases (literal.eval α n) with htt | hff,
-      { apply eval_tt_iff_exists_literal_tt.mpr,
-        use n, simp [mem_cons_self n ns, htt] },
-      { rw count_tt_cons at hne,
-        unfold count_flips at hne,
-        simp [ne_flip_self l, bool.to_nat] at hne,
-        by_cases l = n,
-        { simp [h, ne_flip_self n, hff] at hne,
-          simp [eval_cons, ihred hne, hff] },
-        { have lflip : l.flip = n, from eq_flip_of_eq_var_of_ne h hn.symm,
-          have eflip := eval_flip α l,
-          rw ← lflip at hff,
-          rw hff at eflip,
-          simp [eq_flip_of_eq_var_of_ne h hn.symm, eflip] at hne,
-          simp [eval_cons, ihred hne] } } } }
+  { cases ls;
+    intros c₂ hc₂ hcount,
+    { rcases exists_of_map_singleton hc₂.symm with ⟨n, rfl, hn⟩,
+      cases h : (α l.var),
+      { cases l;
+        rw var at h; 
+        { cases n; rw [var, var] at hn,
+          { simp [h, bool.to_nat, literal.eval, count_flips, literal.flip, hn] at hcount,
+            contradiction },
+          { simp [literal.eval, h, hn] } } },
+      { cases l;
+        rw var at h;
+        { cases n; rw [var, var] at hn,
+          { simp [literal.eval, h, hn] },
+          { simp [h, bool.to_nat, literal.eval, count_flips, literal.flip, hn] at hcount,
+            contradiction } } } },
+    { rcases exists_map_cons_of_map_cons hc₂.symm with ⟨m, ms, rfl, hm, hms⟩,
+      have ihred := ih (cons_ne_nil ls_hd ls_tl) ms hms.symm,
+      cases h : (literal.eval α m),
+      { by_cases he : l = m; rw count_tt_cons at hcount,
+        { simp [h, he, count_flips_cons, bool.to_nat] at hcount,
+          exact eval_tt_cons_of_eval_tt m (ihred hcount) },
+        { have := eval_flip_of_eval h,
+          simp [h, flip_eq_of_ne_of_var_eq (ne.symm he) hm] at this,
+          simp [h, flip_eq_of_ne_of_var_eq he hm.symm, 
+            count_flips_cons, bool.to_nat, this] at hcount,
+          exact eval_tt_cons_of_eval_tt m (ihred hcount) } },
+      { simp [eval_cons, h] } } }
 end
 
-/-! # Grappling with the variables (natural numbers) of the literals of the clause -/
-/- If the below is fully implemented, then it should be refactored everywhere else
+/-! # Clause variables -/
+
+/- Consider changing the implementation to a (fin)set
+
     The motivation for this is twofold
       1. Hide the implementation of clause as a list. Accessing the variables of the clause
          via the below function makes it so that (map var c) doesn't produce the same
       2. Allow for the same in cnf, etc.
- -/
+-/
 
 def vars : clause → list nat
 | []        := []
-| (l :: ls) := l.var :: vars ls
+| (l :: ls) := if l ∈ ls ∨ l.flip ∈ ls then vars ls else l.var :: vars ls
+
+@[simp] theorem vars_nil : vars [] = [] := rfl
+
+@[simp] theorem vars_singleton (l : literal) : vars [l] = [l.var] := 
+by simp [vars]
+
+theorem mem_vars_cons_of_mem_vars {c : clause} (l : literal) : 
+  ∀ {n : nat}, n ∈ vars c → n ∈ vars (l :: c) :=
+assume n hn, by { by_cases (l ∈ c ∨ l.flip ∈ c); simp [vars, h, hn] }
+
+-- This one can probably be cleaned up with a lemma
+theorem mem_vars_of_mem_clause {c : clause} : ∀ {l : literal}, l ∈ c → l.var ∈ vars c :=
+begin
+  induction c with d ds ih,
+  { simp },
+  { intros l hl,
+    rcases eq_or_ne_mem_of_mem hl with rfl | hm,
+    { rcases classical.em (l ∈ ds ∨ l.flip ∈ ds) with ⟨hds | hfds⟩ | h,
+      { simp [ih hds, vars, hds], },
+      { exact flip_var_eq l ▸ mem_vars_cons_of_mem_vars l (ih hfds) },
+      { simp [h, vars] } },
+    { exact mem_vars_cons_of_mem_vars d (ih hm.2) } }
+end
+
+-- Seems a little lengthy in casework
+theorem exists_mem_clause_of_mem_vars {c : clause} {n : nat} : 
+  n ∈ vars c → ∃ (l : literal), l ∈ c ∧ l.var = n :=
+begin
+  induction c with l ls ih,
+  { simp },
+  { by_cases (l ∈ ls ∨ l.flip ∈ ls),
+    { simp [h, vars],
+      intro hn,
+      rcases ih hn with ⟨m, hm, hms⟩,
+      use m, simp [hm, hms] },
+    { simp [h, vars],
+      rintros (hn | hn),
+      { use l, simp [hn] },
+      { rcases ih hn with ⟨m, hm, hms⟩,
+        use m, simp [hm, hms] } } }
+end
+
+theorem vars_subset_of_vars_cons (c : clause) (l : literal) :
+  vars c ⊆ vars (l :: c) :=
+by { by_cases (l ∈ c ∨ l.flip ∈ c); simp [vars, h] }
+
+-- Unsurprisingly, (map var c) and vars c are equivalent from a set perspective
+theorem vars_subset_of_map_var : ∀ (c : clause), vars c ⊆ map var c
+| []        := by simp
+| (l :: ls) := assume n hn, mem_map.mpr (exists_mem_clause_of_mem_vars hn)
+
+theorem map_var_subset_of_vars : ∀ (c : clause), map var c ⊆ vars c
+| []        := by simp
+| (l :: ls) := assume n hn, by 
+  { rcases mem_map.mp hn with ⟨l, hl, hls⟩, exact hls ▸ mem_vars_of_mem_clause hl }
+
+theorem mem_vars_iff_mem_map_vars {c : clause} {n : nat} :
+  n ∈ map var c ↔ n ∈ vars c :=
+⟨λ h, map_var_subset_of_vars c h, λ h, vars_subset_of_map_var c h⟩
+
+theorem not_mem_vars_iff_not_mem_map_vars {c : clause} {n : nat} :
+  n ∉ map var c ↔ n ∉ vars c :=
+by simp [mem_vars_iff_mem_map_vars]
+
+theorem abc {α : Type} [decidable_eq α] {a b : α} {l : list α} : a ∈ l → b ∉ l → a ≠ b :=
+begin
+  library_search,
+end
+
+-- Premises can be curried, but and_imp is being troublesome
+theorem not_mem_vars_of_not_mem_clause {c : clause} {l : literal} : 
+  l ∉ c ∧ l.flip ∉ c → l.var ∉ vars c :=
+begin
+  contrapose,
+  simp,
+  intros hv hc,
+  rcases exists_mem_clause_of_mem_vars hv with ⟨m, hm, hms⟩,
+  exact (flip_eq_of_ne_of_var_eq 
+    (ne.symm (ne_of_mem_of_not_mem hm hc)) hms.symm).symm ▸ hm
+end
+
+theorem vars_nodup (c : clause) : c.vars.nodup :=
+begin
+  induction c with l ls ih,
+  { simp },
+  { simp [vars],
+    rcases (classical.em (l ∈ ls ∨ l.flip ∈ ls)) with ⟨hls | hls⟩ | h,
+    repeat { simp [hls, ih] },
+    { simp [h, ih], 
+      simp [not_or_distrib] at h,
+      rcases h with ⟨h1, h2⟩,
+      exact not_mem_vars_of_not_mem_clause (and.intro h1 h2) } }
+end
 
 def reduced : clause → clause
 | []        := []
 | (l :: ls) := if l ∈ ls then reduced ls else l :: reduced ls
 
 -- TODO can probably be implemented in terms of foldl, foldr
--- TODO Borrow the min_max list derivations for streamlining
+-- TODO Borrow the min_max list derivations for streamlining? Options aren't fun though
 def max_var : clause → nat
 | []        := 0
 | (l :: ls) := max l.var (max_var ls)
@@ -693,7 +793,7 @@ begin
 end
 
 -- Overly situational, I know
-lemma max_var_sublist_append (c₁ c₂ : clause) : ∀ {c₃ : clause}, 
+lemma max_var_sublist_append {c₁ c₂ : clause} : ∀ {c₃ : clause}, 
   c₃ <+ c₁ → max_var c₂ > max_var c₁ → max_var (c₃ ++ c₂) = max_var c₂ :=
 begin
   induction c₁ with d ds ih,
@@ -727,22 +827,69 @@ begin
     exact max_var_sublist (d :: ds) this }
 end
 
-def min_var : clause → nat
-| []        := 1000000 -- Some large number
-| (l :: ls) := min l.var (min_var ls)
+theorem not_mem_of_gt_max_var {c : clause} {l : literal} : l.var > max_var c → l ∉ c :=
+begin
+  induction c with d ds ih,
+  { simp },
+  { intro h,
+    simp [max_var] at h,
+    rcases h with ⟨hd, hds⟩,
+    have : d ≠ l, from ne_of_apply_ne (λ (d : literal), d.var) (ne_of_lt hd),
+    simp [ne.symm this, ih hds] }
+end
 
-/- Alternative defs -/
-def max_var_foldr (c : clause) : nat :=
-  c.foldr (λ l n, max l.var n) 0
+theorem not_mem_map_var_of_gt_max_var {c : clause} {l : literal} : l.var > max_var c → l.var ∉ (map var c) :=
+begin
+  induction c with d ds ih,
+  { simp },
+  { intro h,
+    simp [max_var] at h,
+    rcases h with ⟨hd, hds⟩,
+    simp [hd, ih hds, ne_of_gt hd] }
+end
 
-def min_var_foldr (c : clause) : nat :=
-  c.foldr (λ l n, min l.var n) 1000000
+-- Weird proof
+theorem not_mem_map_var_of_gt_max_var2 {c : clause} {n : nat} : n > max_var c → n ∉ (map var c) :=
+begin
+  intro h,
+  have pos : (Pos n).var = n, simp [var],
+  rw ← pos at h,
+  have := not_mem_map_var_of_gt_max_var h,
+  rw pos at this,
+  exact this
+end
 
-/- Alternative definition 
-   Technically, the empty clause evals to ff, so reduce gives only the two literals
-def reduced : clause → clause
-| []        := []
-| (l :: ls) := if l ∈ ls then (if l.flip ∈ ls then [l, l.flip] else reduced ls) else l :: reduced ls
--/
+theorem not_mem_vars_of_gt_max_var {c : clause} {l : literal} : l.var > max_var c → l.var ∉ c.vars :=
+assume h, not_mem_vars_iff_not_mem_map_vars.mp (not_mem_map_var_of_gt_max_var h)
 
 end clause
+
+/-! # Equivalence on domain for clauses -/
+
+namespace assignment
+
+open assignment
+open list
+open literal
+open clause
+
+theorem eval_eq_of_equiv_on_clause {α₁ α₂ : assignment} {c : clause} :
+  (α₁ ≡[map var c]≡ α₂) → clause.eval α₁ c = clause.eval α₂ c :=
+begin
+  intro heq,
+  cases h : (clause.eval α₂ c),
+  { rw eval_ff_iff_forall_literal_eval_ff at h,
+    apply eval_ff_iff_forall_literal_eval_ff.mpr,
+    intros l hl,
+    exact h l hl ▸ eval_eq_of_mem_of_eqod heq (mem_map_of_mem var hl) },
+  { rcases eval_tt_iff_exists_literal_eval_tt.mp h with ⟨l, hl, hlt⟩,
+    apply eval_tt_iff_exists_literal_eval_tt.mpr,
+    use [l, hl],
+    exact hlt ▸ eval_eq_of_mem_of_eqod heq (mem_map_of_mem var hl) }
+end
+
+theorem eval_eq_of_equiv_on_clause2 {α₁ α₂ : assignment} {c : clause} :
+  (α₁ ≡[vars c]≡ α₂) → clause.eval α₁ c = clause.eval α₂ c :=
+assume h, eval_eq_of_equiv_on_clause (eqod_subset_of_eqod (map_var_subset_of_vars c) h)
+
+end assignment
